untimed/CaseStudy/EvenStream.thy
@@ -1,6 +1,15 @@
+(*  Title:  EvenStream
+    Author: Sebastian Stüber
+    e-mail: sebastian.stueber@rwth-aachen.de
+
+    Description: Part of a case Study for a generated Automaton. 
+      This part only deals with (event) streams, bundles are somewhere else
+*)
+
+
 theory EvenStream
 
-imports "../../untimed/Streams" "../../inc/Event" "Sum"
+imports tsynStream
 
 begin
 
@@ -48,6 +57,7 @@ fun evenMakeSubstate :: "bool \<Rightarrow> EvenAutomatonSubstate" where
 "evenMakeSubstate True = Even" | 
 "evenMakeSubstate False = Odd"
 
+(* transition function for evenAutomaton on event streams *)
 fun evenTransition :: "EvenAutomatonState \<Rightarrow> EvenAutomaton event \<Rightarrow> (EvenAutomaton event \<times> EvenAutomatonState)" where
 "evenTransition s Tick = (Tick, s)" |
 
@@ -62,6 +72,26 @@ abbreviation evenStream:: "EvenAutomaton event stream \<rightarrow> EvenAutomato
 "evenStream \<equiv> sscanlA evenTransition evenInitialState"
 
 
+lemma evenstream_bot: "sscanlA evenTransition state\<cdot>\<bottom> = \<bottom>"
+  by simp
+
+lemma evenstream_tick: "sscanlA evenTransition state\<cdot>(\<up>Tick \<bullet> xs) = \<up>Tick \<bullet> (sscanlA evenTransition state\<cdot>xs)"
+  by simp
+
+lemma evenstream_msg:  "sscanlA evenTransition (State ooo summe) \<cdot>(\<up>(Msg (A m)) \<bullet> xs) 
+    = \<up>(Msg (B (even (summe + m)))) \<bullet> (sscanlA evenTransition (State (evenMakeSubstate (even (summe + m)))  (summe + m))\<cdot>xs)"
+  by simp
+
+
+(* convert the datatypes *)
+abbreviation nat2even:: "nat event stream \<rightarrow> EvenAutomaton event stream" where
+"nat2even \<equiv> tsynMap A"
+
+(* convert the datatypes *)
+abbreviation bool2even:: "bool event stream \<rightarrow> EvenAutomaton event stream" where
+"bool2even \<equiv> tsynMap B"
+
+
 
 (********************************)
     section \<open>Lemma\<close>
@@ -69,10 +99,14 @@ abbreviation evenStream:: "EvenAutomaton event stream \<rightarrow> EvenAutomato
 lemma "#(evenStream\<cdot>s) = #s"
   by simp
 
-(* TODO generalize the smap (\<lambda> m. case m of (Msg n) \<Rightarrow> Msg (B (even n)) | Tick \<Rightarrow> Tick) *)
+lemma evenstream_final_h: "sscanlA evenTransition (State ooo n)\<cdot>(nat2even\<cdot>s) = bool2even\<cdot>(tsynMap even\<cdot>(tsynScanl plus n\<cdot>s))"
+  apply(induction arbitrary: n ooo rule: ind [of _ s])
+    apply auto
+  apply(rename_tac a s n ooo)
+  apply(case_tac a)
+  by auto
 
-lemma "evenStream\<cdot>(smap (\<lambda> m. case m of (Msg n) \<Rightarrow> Msg (A n) | Tick \<Rightarrow> Tick)\<cdot>s) 
-      = smap (\<lambda> m. case m of (Msg n) \<Rightarrow> Msg (B (even n)) | Tick \<Rightarrow> Tick)\<cdot>(sum\<cdot>s)"
-  oops
+lemma evenstream_final: "evenStream\<cdot>(nat2even\<cdot>s) = bool2even\<cdot>(tsynMap even\<cdot>(tsynSum\<cdot>s))"
+  by (simp add: evenInitialState_def tsynSum_def evenstream_final_h)
 
 end
